%% to produce a PDF copy, issue the following command:
%%
%%     pdflatex propositional-logic-examples.tex
%%
%% in the same directory containing the LaTeX style files:
%%
%%     prooftree.sty  and  boxproof.sty

\documentclass[11pt,leqno,fleqn]{article}

\usepackage{graphicx} 
\usepackage{times}              % better fonts for mathematical symbols
\usepackage{bm}                 % unlike \boldmath,
                                % \bm can be used anywhere within math mode
\usepackage[scaled=0.9]{helvet} % makes text a little smaller throughout,
                                % but not the text in math mode.
\usepackage{prooftree}
\usepackage{boxproof}

\usepackage{synttree} 
% \usepackage{bm}


\usepackage{hyperref}



\setlength\hoffset{-5pt}      % horizontal offset, to move text horizontally
\setlength{\textwidth}{4.5in} % try different widths
\setlength\voffset{-5pt}      % vertical offset, to move text vertically
\setlength{\textheight}{7in}  % try different heights

\newcommand{\Hide}[1]{}             % use \Hide{bla bla} to hide ``bla bla''
\newcommand{\code}[1]{\texttt{#1}}  % use \code{...} to produce ASCII chars
\newcommand{\Intro}[1]{{#1}{\textrm{i}}}
\newcommand{\Elim}[1]{{#1}{\textrm{e}}}

\title{CS511 Formal Methods: Homework 01}
\author{Muhammad Faisal} 
\date{} % omit date

\begin{document}

\maketitle


\section{Problem One: Exercise 1.5.7}
\subsection{a}
$$\overline{\phi_1} = (p \land q) \lor ( \overline{p} \land q) \lor (p \land \overline{q})$$
$$\phi_1 = \overline{(p \land q) \lor ( \overline{p} \land q) \lor (p \land \overline{q})}$$
$$\phi_1 = (\overline{p} \lor \overline{q}) \land ( p \lor \overline{q}) \land (\overline{p} \lor q)$$

\subsection{b}
$$\overline{\phi_2} = ( p \land q \land \overline{r} ) \lor ( p \land \overline{q} \land r ) \lor ( p \land \overline{q} \land \overline{r} ) \lor ( \overline{p} \land q \land \overline{r} ) \lor ( \overline{p} \land \overline{q} \land \overline{r})$$
$$\phi_2 = \overline{( p \land q \land \overline{r} ) \lor ( p \land \overline{q} \land r ) \lor ( p \land \overline{q} \land \overline{r} ) \lor ( \overline{p} \land q \land \overline{r} ) \lor ( \overline{p} \land \overline{q} \land \overline{r})}$$
$$\phi_2 = ( \overline{p} \lor \overline{q} \lor r ) \land ( \overline{p} \lor q \lor \overline{r} ) \land ( \overline{p} \lor q \lor r ) \land ( p \lor \overline{q} \lor r ) \land ( p \lor q \lor r)$$

\subsection{c}
$$\overline{\phi_3} = ( r \land s \land q ) \lor ( r \land \overline{s} \land q) \lor ( \overline{r} \land s \land q) \lor ( \overline{r} \land s \land \overline{q}) \lor ( \overline{r} \land \overline{s} \land q)$$
$$\phi_3 = \overline{( r \land s \land q ) \lor ( r \land \overline{s} \land q) \lor ( \overline{r} \land s \land q) \lor ( \overline{r} \land s \land \overline{q}) \lor ( \overline{r} \land \overline{s} \land q)}$$
$$\phi_3 = ( \overline{r} \lor \overline{s} \lor \overline{q} ) \land ( \overline{r} \lor s \lor \overline{q} ) \land ( r \lor \overline{s} \lor \overline{q} ) \land ( r \lor \overline{s} \lor q ) \land ( r \lor s \lor \overline{q} )$$


\section{Problem Two}
\subsection{de Morgan’s Laws:Natural Deduction}
\begin{proofbox}
    \[
       \label{a1}\: \lnot (p \land (q \land r))  \= \textrm{assume} \\
       \[
          \label{a2}\: \lnot(\lnot p \lor (\lnot q \lor \lnot r))  \= \textrm{assume} \\
            \[
                \label{a3}\: \lnot P    \= \textrm{assume}\\
                \label{a4}\: (\lnot p \lor (\lnot q \lor \lnot r))    \= \Intro{\lor}_1\ \ref{a3}\\
                \label{a5}\: \bot    \= \Elim{\lnot}\ \ref{a2},\ref{a4} \\
            \]
            \label{a6}\: \lnot \lnot p    \= \Intro{\lnot}\ \ref{a3}-\ref{a5} \\
            \label{a7}\: p    \= \Elim{}{\lnot{\lnot}}\ \ref{a6} \\
            \[
                \label{a8}\: \lnot q    \= \textrm{assume}\\
                \label{a9}\: (\lnot q \lor \lnot r)    \= \Intro{\lor}_1\ \ref{a8}\\
                \label{a10}\: (\lnot p \lor (\lnot q \lor \lnot r))    \= \Intro{\lor}_9\ \ref{a9}\\
                \label{a11}\: \bot    \= \Elim{\lnot}\ \ref{a2},\ref{a10} \\
            \]
            \label{a12}\: \lnot \lnot q    \= \Intro{\lnot}\ \ref{a8}-\ref{a11} \\
            \label{a13}\: q    \= \Elim{}{\lnot{\lnot}}\ \ref{a12} \\
            \[
                \label{a14}\: \lnot r    \= \textrm{assume}\\
                \label{a15}\: (\lnot q \lor \lnot r)    \= \Intro{\lor}_2\ \ref{a12}\\
                \label{a16}\: (\lnot p \lor (\lnot q \lor \lnot r))    \= \Intro{\lor}_2\ \ref{a15}\\
                \label{a17}\: \bot    \= \Elim{\lnot}\ \ref{a2},\ref{a16} \\
            \]
            \label{a18}\: \lnot \lnot r    \= \Intro{\lnot}\ \ref{a14}-\ref{a17} \\
            \label{a19}\: r    \= \Elim{}{\lnot{\lnot}}\ \ref{a18} \\
            \label{a20}\: q \land r  \= \Intro{\land}\ \ref{a13},\ref{a19} \\
            \label{a21}\:  (p \land (q \land r))  \= \Intro{\land}\ \ref{a7},\ref{a20} \\
            \label{a22}\: \bot    \= \Elim{\lnot}\ \ref{a1},\ref{a21} \\
       \]
       \label{a23}\: \lnot \lnot (\lnot p \lor (\lnot q \lor \lnot r))    \= \Intro{\lnot}\ \ref{a2}-\ref{a22} \\
       \label{a24}\: (\lnot p \lor (\lnot q \lor \lnot r))    \= \Elim{}{\lnot{\lnot}}\ \ref{a23} \\
    \]
    \: \lnot (p \land (q \land r)) \to (\lnot p \lor (\lnot q \lor \lnot r))  \= \Intro{\to}  \\
 \end{proofbox}




% \begin{proofbox}
%     \[
%        \label{a1}\: \lnot (p \land (q \land r))  \= \textrm{assume} \\
%        \[
%             \label{a2}\: \lnot(\lnot p \lor (\lnot q \lor \lnot r))  \= \textrm{assume} \\
%             \[
%                 \label{a3}\: \lnot P    \= \textrm{assume}\\
%                 \label{a4}\: (\lnot p \lor (\lnot q \lor \lnot r))    \= \Intro{\lor{1}}\ \ref{a3}\\
%                 \label{a5}\: \bot    \= \Intro{\land}\ \ref{a5},\ref{a6} \\
%             \]
%             \label{a6}\: \lnot \lnot p    \= \Intro{\land}\ \ref{a5},\ref{a6} \\
%             \label{a7}\: p    \= \Intro{\land}\ \ref{a5},\ref{a6} \\

%             \[
%                 \label{a8}\: \lnot q    \= \Elim{\lor}_1 \ref{a4}\\
%                 \label{a9}\: (\lnot q \lor \lnot r)    \= \Elim{\to}\ \ref{a2}, \ref{a5}\\
%                 \label{a10}\: (\lnot p \lor (\lnot q \lor \lnot r))    \= \Elim{\to}\ \ref{a2}, \ref{a5}\\
%                 \label{a11}\: \bot    \= \Intro{\land}\ \ref{a5},\ref{a6} \\
%             \]
%             \label{a12}\: \lnot \lnot q    \= \Intro{\land}\ \ref{a5},\ref{a6} \\
%             \label{a13}\: q    \= \Intro{\land}\ \ref{a5},\ref{a6} \\

%             \[
%                 \label{a14}\: \lnot r    \= \Elim{\lor}_1 \ref{a4}\\
%                 \label{a15}\: (\lnot q \lor \lnot r)    \= \Elim{\to}\ \ref{a2}, \ref{a5}\\
%                 \label{a16}\: (\lnot p \lor (\lnot q \lor \lnot r))    \= \Elim{\to}\ \ref{a2}, \ref{a5}\\
%                 \label{a17}\: \bot    \= \Intro{\land}\ \ref{a5},\ref{a6} \\
%             \]
%             \: \label{a18}\: \lnot \lnot r    \= \Intro{\land}\ \ref{a5},\ref{a6} \\
%             \label{a19}\: r    \= \Intro{\land}\ \ref{a5},\ref{a6} \\


%             \label{a20}\: q \land r  \= \Intro{\land}\ \ref{a5},\ref{a6} \\


%             \label{a21}\: P\land Q    \= \Intro{\land}\ \ref{a4},\ref{a5}-\ref{a7},\ref{a8}-\ref{a10} \\
%        \]
%        \label{a22}\: \not \not (\lnot p \lor (\lnot q \lor \lnot r))    \= \Elim{\lor}\ \ref{a1},\ref{a2} \\
%        \label{a23}\: (\lnot p \lor (\lnot q \lor \lnot r))    \= \Elim{\lor}\ \ref{a1},\ref{a2} \\
%     \]
%     \: \lnot (p \land (q \land r)) \to (\lnot p \lor (\lnot q \lor \lnot r))  \= \Intro{\to}  \\
%  \end{proofbox}


\subsection{de Morgan’s Laws:Analytic Tableaux}
Since the negation of the de Morgan's law is a contradiction (not satisfiable), the law is a tautology.
\begin{center}
   \synttree{8 \branchheight{.45in} \childsidesep{5em} \childattachsep{1em}}
   [ $\Gamma = \{\lnot(\lnot (p \land (q \land r)) \to (\lnot p \lor (\lnot q \lor \lnot r)))\}$ 
      [
         $\lnot (p \land (q \land r))$ [
            $\lnot (\lnot p \lor (\lnot q \lor \lnot r))$[
               $\lnot \lnot p$ [
                  $\lnot (\lnot q \lor \lnot r)$
                  [$\lnot p$[
                     $\lnot \lnot q$[
                              $\lnot \lnot r$ [
                                 $p$
                              ]
                           ]
                  ]]
                  [$\lnot (q \land r)$[
                     $\lnot q$ [
                        $\lnot r$[
                           $\lnot \lnot q$[
                              $\lnot \lnot r$ [
                                 $r$
                              ]
                           ]
                        ]
                     ]
                  ]]
               ]
            ]
         ]
      ]
   ]
   \end{center}




   % $\lnot (p \land (q \land r)) \to (\lnot p \lor (\lnot q \lor \lnot r))$
   % [$\lnot \lnot (p \land (q \land r))$[
   %    $(p \land (q \land r))$
   %       [$p$[$(q \land r)$ [$q$[$r$]]]
   %    ]
   % ]]
   % [$(\lnot p \lor (\lnot q \lor \lnot r))$
   %    [$\lnot p$]
   %    [$(\lnot q \lor \lnot r)$
   %    [$\lnot q$]
   %    [$\lnot r$]
   %    ]
   % ]

% \section{Problem One}

% \subsection{DNF of majority function}
% $\phi = (\lnot z \land y \land x) \lor (z \land \lnot y \land x) \lor (z \land y \land \lnot x) \lor (z \land y \land x) $

% \subsection{CNF of majority function}
% $\psi = (\lnot z \lor y \lor x) \land (z \lor \lnot y \lor x) \land (z \lor y \lor \lnot x) \land (z \lor y \lor x) $

% \subsection{Checking with Z3 script}

% \begin{verbatim}
%    (declare-const x Bool)
%    (declare-const y Bool)
%    (declare-const z Bool)
   
%    (declare-fun phi (Bool Bool Bool) Bool)
%    (assert (= (phi x y z)
%               (or (and x (and y (not z))) (or (and x (and (not y) z))
%                 (or (and (and (not x) y) z) (and (and x y) z) ) ))))
   
%    (declare-fun psi (Bool Bool Bool) Bool)
%    (assert (= (psi x y z)
%               (and (or x (or y (not z))) (and (or x (or (not y) z))
%                 (and (or (or (not x) y) z) (or (or x y) z) ) ))))
   
%    (assert ( = (phi x y z) (psi x y z)))
   
%    (check-sat)
% \end{verbatim}


% \subsection{Checking with Z3Py script}
% \begin{verbatim}
%    from z3 import *

%    x,y,z = Bools('x y z')

%    phi = Or (And(Not(z),y,x), And(z,Not(y),x), And(z,y,Not(x)), And(z,y,x))

%    psi = And (Or(Not(z),y,x), Or(z,Not(y),x), Or(z,y,Not(x)), Or(z,y,x)) 

%    s = Solver()
%    s.add((phi == psi))

%    print s.check()
% \end{verbatim}


% \pagebreak

% \section{Problem Two}
% Prove the following theorems of propositional logic:

% \subsection{$((P \to Q) \to Q) \to ((Q \to P) \to P)$}

% % \begin{proofbox}
% %     \[
% %        \label{a1}\: ((P \to Q) \to Q)  \= \textrm{assume} \\
% %        \: P\land Q    \= \Intro{\land}\ \ref{a1},\ref{a2} \\
% %     \]
% %     \: Q\to(P\land Q) \= \Intro{\to}  \\
% %  \end{proofbox}



% \subsection{$((P \to Q) \land (Q \to P)) \to ((P \lor Q) \to (P \land Q)) $}

% \begin{proofbox}
%     \[
%        \label{a1}\: (P \to Q) \land (Q \to P)  \= \textrm{assume} \\
%        \label{a2}\: P \to Q    \= \Elim{\land}_1\ \ref{a1}\\
%        \label{a3}\: Q \to P    \= \Elim{\land}_2\ \ref{a1}\\
%        \[
%             \label{a4}\: P \lor Q  \= \textrm{assume} \\
%             \[
%                 \label{a5}\: P    \= \Elim{\lor}_1 \ref{a4}\\
%                 \label{a6}\: Q    \= \Elim{\to}\ \ref{a2}, \ref{a5}\\
%                 \label{a7}\: P \land Q    \= \Intro{\land}\ \ref{a5},\ref{a6} \\
%             \]
%             \[
%                 \label{a8}\: Q    \= \Elim{\lor}_2 \ref{a4}\\
%                 \label{a9}\: P    \= \Elim{\to}\ \ref{a3}, \ref{a8}\\
%                 \label{a10}\: P \land Q    \= \Intro{\land}\ \ref{a8},\ref{a9} \\
%             \]
%             \: P\land Q    \= \Intro{\land}\ \ref{a4},\ref{a5}-\ref{a7},\ref{a8}-\ref{a10} \\
%        \]
%        \: ((P \lor Q) \to (P \land Q))    \= \Elim{\lor}\ \ref{a1},\ref{a2} \\
%     \]
%     \: ((P \to Q) \land (Q \to P)) \to ((P \lor Q) \to (P \land Q))  \= \Intro{\to}  \\
%  \end{proofbox}




% \subsection{$(P \to Q) \to ( (\lnot P \to Q) \to Q)$}
% \begin{proofbox}
%     \[
%        \label{a1}\: P \to Q  \= \textrm{assume} \\
%        \[
%             \label{a2}\: \lnot P \to Q  \= \textrm{assume} \\
%             \[
%                 \label{a3}\: \lnot Q    \= \textrm{assume}\\
%                 \label{a4}\: \lnot \lnot P    \= \textrm{MT} \ \ref{a2},\ref{a3}\\
%                 \label{a5}\: P    \= \Elim{\neg{\neg{}}} \ \ref{a4}\\
%                 \label{a6}\: Q    \= \Elim{\to}\ \ref{a1}, \ref{a5}\\
%                 \label{a7}\: \lnot \lnot Q    \= \Intro{}{\neg{\neg}} \ \ref{a6}\\
%                 \label{a8}\: \bot    \= \Elim{\neg}\ \ref{a3}, \ref{a7}\\
%             \]
%             \: Q    \= \textrm{PBC} \ \ref{a3}-\ref{a8} \\
%        \]
%        \: (\lnot P \to Q) \to Q    \= \Intro{\to}  \ \ref{a2}-\ref{a9}\\
%     \]
%     \: (P \to Q) \to ( (\lnot P \to Q) \to Q)  \= \Intro{\to}  \\
%  \end{proofbox}



% \pagebreak



% \section{Problem 04}

% \begin{enumerate}
%    \item $\Intro{\lnot}$ : $\phi \to \bot$
%    \item $\Elim{\lnot}$ : $\frac {\phi} {\bot \to \phi}$
%    \item $\Intro{\lnot{\lnot}}$ : $(\phi \to \bot) \to  \bot$
%    \item $\Elim{\lnot{\lnot}}$ : $\frac{\phi} {(\bot \to \phi) \to \phi} $
% \end{enumerate}


% \section{Problem 05}
% \subsection{adequate sets}
%    The following explain why which one can be adequeate set.
% \begin{enumerate}
%    \item $\{\lnot \ , \land\}$: $\phi \to \psi \equiv \lnot (\phi \land \lnot \psi)$, $ ( \phi \land \psi ) \equiv (\lnot (\lnot \phi \lor \lnot \psi)) $
%    \item $\{\lnot \ , \to\}$: $(\phi \land \psi) \equiv (\phi \to \psi, \psi \to phi)$,  $(\phi \lor \psi) \equiv \phi \to \lnot \psi$
%    \item $\{\to \ , \bot\}$: $\lnot p \equiv p \to \bot $, $(\phi \lor \lnot \psi) \equiv \phi \to \psi$ 
% \end{enumerate}

% \subsection{b}
% Without either $\lnot$, $\bot$, the symbols can not express all situations. For example, the truth table for such expressions with these symbols would have only the case when all variables are set to 1 because negation is not a possible case for any variable.

% \subsection{C}
% They are not adequate because they can only express tautologies. For example, the $p \to q$ can not be expressed using these symbols.





\pagebreak
\section{Problem 05}
\href{https://github.com/mickey-me/CS511_formal_methods/blob/master/assignments/assignment02/P5.smt2}{Click here for Code file}
or copy the following link:
\url{https://github.com/mickey-me/CS511_formal_methods/blob/master/assignments/assignment02/P5.smt2}


\section{Problem 06}
\href{https://github.com/mickey-me/CS511_formal_methods/blob/master/assignments/assignment02/P6.py}{Click here for Code file}
or copy the following link:
\url{https://github.com/mickey-me/CS511_formal_methods/blob/master/assignments/assignment02/P6.py}




% \section{Problem 06}

% \section{Example: $P \vdash Q\to(P\land Q)$}

% \begin{proofbox}
%    \label{a1}\: P \= \textrm{premise} \\
%    \[
%       \label{a2}\: Q  \= \textrm{assume} \\
%       \: P\land Q    \= \Intro{\land}\ \ref{a1},\ref{a2} \\
%    \]
%    \: Q\to(P\land Q) \= \Intro{\to}  \\
% \end{proofbox}

% \section{Example: $P\to(Q\to R) \vdash P\land Q\to R$}

% \begin{proofbox}
%    \label{b1}\: P\to(Q\to R) \= \textrm{premise} \\
%    \[
%       \label{b2}\: P\land Q    \= \textrm{assume} \\
%       \label{b3}\: P \= {\Elim{\land}}_1\ \ \ref{b2}\\
%       \label{b4}\: Q\to R \= \Elim{\to}\ \ \ref{b1},\ref{b3}\\
%       \label{b5}\: Q \= {\Elim{\land}}_2\ \ \ref{b2}\\
%       \: R \=\Elim{\to}\ \ \ref{b4},\ref{b5}\\
%    \]
%       \: P\land Q\to R \= \Intro{\to} \\
% \end{proofbox}

% \section{Example: $P\land Q\to R \vdash P\to(Q\to R)$}

% \begin{proofbox}
%    \label{c1}\: P\land Q\to R \= \textrm{premise} \\
%    \[
%       \label{c2}\: P     \= \textrm{assume} \\
%       \[
%          \label{c3}\: Q  \= \textrm{assume} \\
%          \label{c4}\: P\land Q \= \Intro\land\ \ref{c2},\ref{c3}\\
%          \: R \= \Elim\to\ \ref{c1},\ref{c4}
%       \]
%       \: Q\to R \= \Intro\to \\
%    \]
%    \: P\to(Q\to R) \= \Intro\to \\
% \end{proofbox}

% \section{Example: $P\to(Q\to R) \vdash (P\to Q)\to(P\to R)$}

% \begin{proofbox}
%    \label{d1}\: P\to(Q\to R) \= \textrm{premise} \\
%    \[
%       \label{d2}\: P\to Q  \= \textrm{assume} \\
%       \[
%          \label{d3}\: P    \= \textrm{assume} \\
%          \label{d4}\: Q \= \Elim\to\ \ref{d2},\ref{d3}\\
%          \label{d5}\: Q\to R \= \Elim\to \ref{d1},\ref{d3}\\
%          \: R \= \Elim\to\ \ref{d5},\ref{d4}\\
%       \]
%       \: P\to R \= \Intro\to \\
%    \]
%    \: (P\to Q)\to(P\to R) \= \Intro\to \\
% \end{proofbox}

% \section{Example:  $\quad P\land\neg{Q}\to R,\ \ \neg{R},\ \ P \quad\vdash\quad Q$}

% \begin{proofbox}
%    \label{aa}\: P\land\neg{Q}\to R \= \textrm{premise}\\
%    \label{bb}\: \neg{R} \= \textrm{premise}\\
%    \label{cc}\: P \= \textrm{premise}\\
%    \[
%       \label{dd}\: \neg{Q} \= \textrm{assume}\\
%       \label{ee}\: P\land\neg{Q} \= {\Intro{\land}}\ \ \ref{cc},\ref{dd}\\
%       \label{ff}\: R \= \Elim{\to}\ \ \ref{aa},\ref{ee}\\
%       \label{gg}\: \bot \= {\Elim{\neg{}}}\ \ \ref{ff},\ref{bb}\\
%    \]
%       \label{hh}\: \neg{\neg{Q}} \= \Intro{\neg{}} \\
%       \: Q \= \Elim{\neg{\neg{}}}\ \ \ref{hh} \\
% \end{proofbox}




\end{document}

